Logic/Predicate/FirstOrder/Hauptsatz.lean
@@ -58,7 +58,7 @@ def andInversion₁Aux : {Δ : Sequent L} → (d : ⊢ᶜ[P] Δ) → (p q : Synt
         (by simp[shifts_insert, shifts_erase, Finset.subset_iff]; rintro x hx (rfl | hhx) <;> simp[*])
     (all _ _ this).cast (by simp[Finset.erase_insert_of_ne, Finset.Insert.comm p])
   | _, ex Δ t r d,          p, q =>
-    have : ⊢ᶜ[P] insert (subst t r) (insert p $ Δ.erase (p ⋏ q)) :=
+    have : ⊢ᶜ[P] insert (⟦↦ t⟧ r) (insert p $ Δ.erase (p ⋏ q)) :=
       (andInversion₁Aux d p q).weakening (by simp[Finset.subset_iff]; rintro x hx (rfl | hhx) <;> simp[*])
     (ex _ t r this).cast (by simp[Finset.erase_insert_of_ne, Finset.Insert.comm p])
   | _, cut Δ Γ r hr dΔ dΓ,  p, q =>
@@ -94,7 +94,7 @@ def andInversion₂Aux : {Δ : Sequent L} → ⊢ᶜ[P] Δ → (p q : SyntacticF
         (by simp[shifts_insert, shifts_erase, Finset.subset_iff]; rintro x hx (rfl | hhx) <;> simp[*])
     (all _ _ this).cast (by simp[Finset.erase_insert_of_ne, Finset.Insert.comm q])
   | _, ex Δ t r d,          p, q =>
-    have : ⊢ᶜ[P] insert (subst t r) (insert q $ Δ.erase (p ⋏ q)) :=
+    have : ⊢ᶜ[P] insert (⟦↦ t⟧ r) (insert q $ Δ.erase (p ⋏ q)) :=
       (andInversion₂Aux d p q).weakening (by simp[Finset.subset_iff]; rintro x hx (rfl | hhx) <;> simp[*])
     (ex _ t r this).cast (by simp[Finset.erase_insert_of_ne, Finset.Insert.comm q])
   | _, cut Δ Γ r hr dΔ dΓ,  p, q =>
@@ -108,47 +108,47 @@ def andInversion₂ {p q} (d : ⊢ᶜ[P] insert (p ⋏ q) Δ) : ⊢ᶜ[P] insert
   (andInversion₂Aux d p q).weakening (by simp; exact Finset.insert_subset_insert _ (Finset.erase_subset _ _))
 
 def allInversionAux : {Δ : Sequent L} → ⊢ᶜ[P] Δ →
-    (p : SyntacticSubFormula L 1) → (t : SyntacticTerm L) → ⊢ᶜ[P] insert (subst t p) (Δ.erase (∀' p))
+    (p : SyntacticSubFormula L 1) → (t : SyntacticTerm L) → ⊢ᶜ[P] insert (⟦↦ t⟧ p) (Δ.erase (∀' p))
   | _, axL Δ r v hpos hneg, p, t => axL _ r v (by simp[hpos]) (by simp[hneg])
   | _, verum Δ h,           p, t => verum _ (by simp[h])
   | _, and Δ r s dr ds,     p, t =>
-      have dr : ⊢ᶜ[P] (insert r $ insert (subst t p) $ Δ.erase (∀' p)) :=
+      have dr : ⊢ᶜ[P] (insert r $ insert (⟦↦ t⟧ p) $ Δ.erase (∀' p)) :=
         (allInversionAux dr p t).weakening (by simp[Finset.subset_iff]; rintro x hx (rfl | hhx) <;> simp[*])
-      have ds : ⊢ᶜ[P] (insert s $ insert (subst t p) $ Δ.erase (∀' p)) :=
+      have ds : ⊢ᶜ[P] (insert s $ insert (⟦↦ t⟧ p) $ Δ.erase (∀' p)) :=
         (allInversionAux ds p t).weakening (by simp[Finset.subset_iff]; rintro x hx (rfl | hhx) <;> simp[*])
       (and _ _ _ dr ds).cast (by simp[Finset.erase_insert_of_ne, Finset.Insert.comm])
   | _, or Δ r s d,          p, t =>
-      have : ⊢ᶜ[P] (insert r $ insert s $ insert (subst t p) $ Δ.erase (∀' p)) :=
+      have : ⊢ᶜ[P] (insert r $ insert s $ insert (⟦↦ t⟧ p) $ Δ.erase (∀' p)) :=
         (allInversionAux d p t).weakening (by simp[Finset.subset_iff]; rintro x hx (rfl | rfl | hhx) <;> simp[*])
       (or _ _ _ this).weakening (by simp[Finset.erase_insert_of_ne, Finset.Insert.comm])
   | _, all Δ p' d,          p, t => by
       by_cases e : p' = p
       · simp[e]
-        let d' : ⊢ᶜ[P] insert (subst t p) Δ :=
-          (d.rewrite hP (t :>ₙ SubTerm.fvar)).cast (by simp[rewrite_free_eq_subst, rewrite_shift_eq_self, shifts_eq_image, Finset.image_image, Function.comp, e])
+        let d' : ⊢ᶜ[P] insert (⟦↦ t⟧ p) Δ :=
+          (d.rewrite hP (t :>ₙ SubTerm.fvar)).cast (by simp[rewrite_free_eq_substs, rewrite_shift_eq_self, shifts_eq_image, Finset.image_image, Function.comp, e])
         have : d'.length = d.length := by simp
         exact (allInversionAux d' p t).weakening (by simp[Finset.subset_iff]; rintro x hx (rfl | hhx) <;> simp[*])
       · have ne : ∀' p' ≠ ∀' p := by simpa using e
-        have : ⊢ᶜ[P] (insert (free p') $ shifts $ insert (subst t p) $ Δ.erase (∀' p)) :=
+        have : ⊢ᶜ[P] (insert (free p') $ shifts $ insert (⟦↦ t⟧ p) $ Δ.erase (∀' p)) :=
           (allInversionAux d (shift p) t.shift).weakening (by
-            simp[shift_subst, shifts_insert, shifts_erase, Finset.subset_iff]; rintro x hx (rfl | hx) <;> simp[*])
+            simp[shift_substs1, shifts_insert, shifts_erase, Finset.subset_iff]; rintro x hx (rfl | hx) <;> simp[*])
         exact (all _ p' this).cast (by simp[Finset.erase_insert_of_ne ne, Finset.Insert.comm])
   | _, ex Δ u q d,          p, t =>
-    have : ⊢ᶜ[P] (insert (subst u q) $ insert (subst t p) $ Δ.erase (∀' p)) :=
+    have : ⊢ᶜ[P] (insert (⟦↦ u⟧ q) $ insert (⟦↦ t⟧ p) $ Δ.erase (∀' p)) :=
       (allInversionAux d p t).weakening (by simp[Finset.subset_iff]; rintro x hx (rfl | hhx) <;> simp[*])
     ((ex _ u q this).cast (by simp[Finset.erase_insert_of_ne, Finset.Insert.comm]))
   | _, cut Δ Γ r hr dΔ dΓ,  p, t =>
-    have dΔ : ⊢ᶜ[P] (insert r $ insert (subst t p) $ Δ.erase (∀' p)) :=
+    have dΔ : ⊢ᶜ[P] (insert r $ insert (⟦↦ t⟧ p) $ Δ.erase (∀' p)) :=
       (allInversionAux dΔ p t).weakening (by simp[Finset.subset_iff]; rintro x hx (rfl | hhx) <;> simp[*])
-    have dΓ : ⊢ᶜ[P] (insert (~r) $ insert (subst t p) $ Γ.erase (∀' p)) :=
+    have dΓ : ⊢ᶜ[P] (insert (~r) $ insert (⟦↦ t⟧ p) $ Γ.erase (∀' p)) :=
       (allInversionAux dΓ p t).weakening (by simp[Finset.subset_iff]; rintro x hx (rfl | hhx) <;> simp[*])
     (cut _ _ r hr dΔ dΓ).cast (by simp[Finset.erase_union])
   termination_by allInversionAux _ d _ _ => d.length
 
-def allInversion (d : ⊢ᶜ[P] insert (∀' p) Δ) (t) : ⊢ᶜ[P] insert (subst t p) Δ :=
+def allInversion (d : ⊢ᶜ[P] insert (∀' p) Δ) (t) : ⊢ᶜ[P] insert (⟦↦ t⟧ p) Δ :=
   (allInversionAux hP d p t).weakening (by simp; exact Finset.insert_subset_insert _ (Finset.erase_subset _ _))
 
-def allInversionClx {i} (d : ⊢ᶜ[< i] insert (∀' p) Δ) (t) : ⊢ᶜ[< i] insert (subst t p) Δ :=
+def allInversionClx {i} (d : ⊢ᶜ[< i] insert (∀' p) Δ) (t) : ⊢ᶜ[< i] insert (⟦↦ t⟧ p) Δ :=
   allInversion (by simp) d t
 
 def falsumElimAux : {Δ : Sequent L} → ⊢ᶜ[P] Δ → ⊢ᶜ[P] Δ.erase ⊥
@@ -168,7 +168,7 @@ def falsumElimAux : {Δ : Sequent L} → ⊢ᶜ[P] Δ → ⊢ᶜ[P] Δ.erase ⊥
         (by {simp[Finset.subset_iff, shifts_eq_image]; rintro x hx (rfl | ⟨y, hy, rfl⟩); { exact Or.inl rfl }; { exact Or.inr ⟨y, ⟨by rintro rfl; contradiction, hy⟩, rfl⟩ } } )
     (all _ _ this).cast (by simp[Finset.erase_insert_of_ne])
   | _, ex Δ t p d          =>
-    have : ⊢ᶜ[P] (insert (subst t p) $ Δ.erase ⊥) := d.falsumElimAux.weakening (by simp[Finset.subset_iff]; rintro x hx (rfl | hhx) <;> simp[*])
+    have : ⊢ᶜ[P] (insert (⟦↦ t⟧ p) $ Δ.erase ⊥) := d.falsumElimAux.weakening (by simp[Finset.subset_iff]; rintro x hx (rfl | hhx) <;> simp[*])
     (ex _ t p this).cast (by simp[Finset.erase_insert_of_ne])
   | _, cut Δ Γ p hp dΔ dΓ  =>
     have dΔ : ⊢ᶜ[P] (insert p $ Δ.erase ⊥) := dΔ.falsumElimAux.weakening (by simp[Finset.subset_iff]; rintro x hx (rfl | hhx) <;> simp[*])
@@ -227,15 +227,15 @@ def reductionAux {i} : {Δ : Sequent L} →
       exact this.cast (by simp[e, Finset.erase_insert_of_ne (Ne.symm e)])
   | _, ex Δ t q d₁,          p, tp, hp, Γ, d₂ => by
     by_cases e : p = ∃' q
-    · have d₁₁ : ⊢ᶜ[< i] (insert (subst t q) $ (Δ.erase (∃' q) ∪ Γ)) :=
+    · have d₁₁ : ⊢ᶜ[< i] (insert (⟦↦ t⟧ q) $ (Δ.erase (∃' q) ∪ Γ)) :=
         (reductionAux d₁ tp hp d₂).cast (by simp[e, Finset.erase_insert_of_ne])
-      have d₂₁ : ⊢ᶜ[< i] (insert (~subst t q) Γ) :=
+      have d₂₁ : ⊢ᶜ[< i] (insert (~⟦↦ t⟧ q) Γ) :=
         by simpa using allInversionClx (p := ~q) (by simpa[e] using d₂) t
       have : ⊢ᶜ[< i] Δ.erase (∃' q) ∪ Γ :=
-        (cut (Δ.erase (∃' q) ∪ Γ) Γ (subst t q)
-          (by simp[subst]; exact Nat.succ_le.mp (by simpa[e] using hp)) d₁₁ d₂₁).cast (by simp)
+        (cut (Δ.erase (∃' q) ∪ Γ) Γ (⟦↦ t⟧ q)
+          (by simp[substs]; exact Nat.succ_le.mp (by simpa[e] using hp)) d₁₁ d₂₁).cast (by simp)
       exact this.cast (by simp[e])
-    · have : ⊢ᶜ[< i] (insert (subst t q) $ Δ.erase p ∪ Γ) :=
+    · have : ⊢ᶜ[< i] (insert (⟦↦ t⟧ q) $ Δ.erase p ∪ Γ) :=
         (reductionAux d₁ tp hp d₂).weakening (by simp[Finset.subset_iff]; rintro x (⟨hxp, (rfl | hhxp)⟩ | hhx) <;> simp[*])
       have : ⊢ᶜ[< i] (insert (∃' q) $ Δ.erase p ∪ Γ) := ex _ t q this
       exact this.cast (by simp[Finset.erase_insert_of_ne (Ne.symm e)])
