Logic/Predicate/Meta.lean
@@ -10,122 +10,75 @@ namespace Meta
 section lemmata
 variable {L : Language.{u}} {μ : Type v} {n}
 
+section substs
+
+lemma substs_bvar_of_eq {n n'} {w : Fin n → SubTerm L μ n'} {x : Fin n} {t} (h : w x = t) :
+    substs w #x = t :=
+  by simp[h]
+
+lemma substs_func_of_eq {n n'} {w : Fin n → SubTerm L μ n'} {k} (f : L.func k) {v : Fin k → SubTerm L μ n} {v'} (h : substs w ∘ v = v') :
+    substs w (func f v) = func f v' :=
+  by simp[substs_func, Function.comp, ←h]
+
+lemma substs_substs_of_eq {l k n} {v : Fin l → SubTerm L μ k} {w : Fin k → SubTerm L μ n}
+  {t : SubTerm L μ l} {v'} {t'}
+  (hv : substs w ∘ v = v') (ht : substs v' t = t') :
+    substs w (substs v t) = t' := by simp[substs_substs, ←hv, ←ht]
+
+lemma substs_eq_of_eq {k n} {w w' : Fin k → SubTerm L μ n} {t t' : SubTerm L μ k} {u}
+  (hw : w = w') (ht : t = t') (h : substs w' t' = u) : substs w t = u := hw ▸ ht ▸ h
+
+end substs
+
+section shift
+
+lemma shift_func_of_eq {n} (f : L.func k) {v : Fin k → SyntacticSubTerm L n} {v'} (h : shift ∘ v = v') :
+    shift (func f v) = func f v' :=
+  by simp[shift_func, Function.comp, ←h]
+
+lemma shift_substs_of_eq {t : SyntacticSubTerm L k} {w : Fin k → SyntacticSubTerm L n} {t' t'' w'}
+  (ht : shift t = t') (hw : shift ∘ w = w') (ht' : substs w' t' = t'') :
+    shift (substs w t) = t'' := by
+  simp[←ht, ←hw, ←ht', shift, substs, map, bind_bind]
+
+end shift
+
+section bShift
+
+lemma bShift_func_of_eq (f : L.func k) {v : Fin k → SubTerm L μ n} {v'} (h : bShift ∘ v = v'):
+    bShift (func f v) = func f v' := by simp[←h, bShift_func]; funext x; simp
+
+lemma bShift_substs_of_eq {w : Fin k → SubTerm L μ n} {t : SubTerm L μ k} {w' t'}
+  (hw : bShift ∘ w = w') (ht : substs w' t = t') :
+    bShift (substs w t) = t' := by
+  simp[←hw, ←ht, bShift, substs, map, bind_bind]; congr
+
+end bShift
+
+section free
+
 lemma free_bvar_last (n : ℕ) : free (#⟨n, Nat.lt.base n⟩ : SyntacticSubTerm L (n + 1)) = &0 :=
   SubTerm.free_bvar_last
 
 lemma free_bvar_of_lt (x : Fin (n + 1)) (h : x.val < n) : free (#x : SyntacticSubTerm L (n + 1)) = #⟨x, h⟩ :=
   free_bvar_castSucc (L := L) ⟨x, h⟩
 
-lemma free_func0 (f : L.func 0) :
-    SubTerm.free (SubTerm.func (L := L) (n := n + 1) f ![]) = SubTerm.func f ![] := by simp[free_func]
+lemma free_func_of_eq {n} (f : L.func k) {v : Fin k → SyntacticSubTerm L (n + 1)} {v'} (h : free ∘ v = v') :
+    free (func f v) = func f v' :=
+  by simp[free_func, Function.comp, ←h]
 
-lemma free_func1 (f : L.func 1) {t : SyntacticSubTerm L (n + 1)} {t'} (h : free t = t'):
-    SubTerm.free (SubTerm.func f ![t]) = SubTerm.func f ![t'] := by simp[←h, free_func]; funext x; simp
+lemma free_substs_of_eq {t : SyntacticSubTerm L k} {w : Fin k → SyntacticSubTerm L (n + 1)} {t' w' t''}
+  (ht : shift t = t') (hw : free ∘ w = w') (ht' : substs w' t' = t'') :
+    free (substs w t) = t'' := by
+  simp[←ht, ←hw, ←ht', shift, map, free, substs, bind_bind]
 
-lemma free_func2 (f : L.func 2) {t₁ t₂ : SyntacticSubTerm L (n + 1)} {t₁' t₂'}
-  (h₁ : free t₁ = t₁') (h₂ : free t₂ = t₂') :
-    SubTerm.free (SubTerm.func f ![t₁, t₂]) = SubTerm.func f ![t₁', t₂'] :=
-  by simp[←h₁, ←h₂, free_func]; funext x; cases x using Fin.cases <;> simp
+end free
 
-lemma free_func3 (f : L.func 3) {t₁ t₂ t₃ : SyntacticSubTerm L (n + 1)} {t₁' t₂' t₃'}
-  (h₁ : free t₁ = t₁') (h₂ : free t₂ = t₂') (h₃ : free t₃ = t₃') :
-    SubTerm.free (SubTerm.func f ![t₁, t₂, t₃]) = SubTerm.func f ![t₁', t₂', t₃'] := by
-  simp[←h₁, ←h₂, ←h₃, free_func]; funext x;
-  cases' x using Fin.cases with x <;> simp;
-  cases' x using Fin.cases with x <;> simp
-
-lemma subst_bvar_last (n : ℕ) (s : SubTerm L μ n) :
-    subst s (#⟨n, Nat.lt.base n⟩ : SubTerm L μ (n + 1)) = s :=
-  SubTerm.subst_bvar_last _
-
-lemma subst_bvar_of_lt {s : SubTerm L μ n} (x : Fin (n + 1)) (h : x.val < n) : 
-    subst s (#x : SubTerm L μ (n + 1)) = #⟨x, h⟩ :=
-  subst_bvar_castSucc s ⟨x, h⟩
-
-lemma subst_func0 {s : SubTerm L μ n} (f : L.func 0) :
-    subst s (SubTerm.func (L := L) (n := n + 1) f ![]) = SubTerm.func f ![] := by simp[subst_func]
-
-lemma subst_func1 {s : SubTerm L μ n} (f : L.func 1) {t : SubTerm L μ (n + 1)} {t'} (h : subst s t = t'):
-    subst s (SubTerm.func f ![t]) = SubTerm.func f ![t'] := by simp[←h, subst_func]; funext x; simp
-
-lemma subst_func2 {s : SubTerm L μ n} (f : L.func 2) {t₁ t₂ : SubTerm L μ (n + 1)} {t₁' t₂'}
-  (h₁ : subst s t₁ = t₁') (h₂ : subst s t₂ = t₂') :
-    subst s (SubTerm.func f ![t₁, t₂]) = SubTerm.func f ![t₁', t₂'] :=
-  by simp[←h₁, ←h₂, subst_func]; funext x; cases x using Fin.cases <;> simp
-
-lemma subst_func3 {s : SubTerm L μ n} (f : L.func 3) {t₁ t₂ t₃ : SubTerm L μ (n + 1)} {t₁' t₂' t₃'}
-  (h₁ : subst s t₁ = t₁') (h₂ : subst s t₂ = t₂') (h₃ : subst s t₃ = t₃') :
-    subst s (SubTerm.func f ![t₁, t₂, t₃]) = SubTerm.func f ![t₁', t₂', t₃'] := by
-  simp[←h₁, ←h₂, ←h₃, subst_func]; funext x;
-  cases' x using Fin.cases with x <;> simp;
-  cases' x using Fin.cases with x <;> simp
-
-lemma shift_func0 (f : L.func 0) :
-    shift (SubTerm.func (L := L) (n := n) f ![]) = SubTerm.func f ![] := by simp[shift_func]
-
-lemma shift_func1 (f : L.func 1) {t t' : SyntacticSubTerm L n} (h : shift t = t'):
-    shift (SubTerm.func f ![t]) = SubTerm.func f ![t'] := by simp[shift_func, ←h]; funext x; simp
-
-lemma shift_func2 (f : L.func 2) {t₁ t₂ t₁' t₂' : SyntacticSubTerm L n}
-  (h₁ : shift t₁ = t₁') (h₂ : shift t₂ = t₂') :
-    shift (SubTerm.func f ![t₁, t₂]) = SubTerm.func f ![t₁', t₂'] :=
-  by simp[shift_func, ←h₁, ←h₂]; funext x; cases x using Fin.cases <;> simp
-
-lemma shift_func3 (f : L.func 3) {t₁ t₂ t₃ t₁' t₂' t₃' : SyntacticSubTerm L n}
-  (h₁ : shift t₁ = t₁') (h₂ : shift t₂ = t₂') (h₃ : shift t₃ = t₃') :
-    shift (SubTerm.func f ![t₁, t₂, t₃]) = SubTerm.func f ![t₁', t₂', t₃'] := by
-  simp[shift_func, ←h₁, ←h₂, ←h₃]; funext x;
-  cases' x using Fin.cases with x <;> simp;
-  cases' x using Fin.cases with x <;> simp
-
-lemma shift_subst {t : SyntacticSubTerm L (n + 1)} {u t' u'}
-  (ht : shift t = t') (hu : shift u = u') :
-    shift (subst u t) = subst u' t' := by
-  simp[←ht, ←hu, shift, SubTerm.subst, map, bind_bind]; congr; funext x
-  cases' x using Fin.lastCases with x <;> simp
-
-lemma bShift_func0 (f : L.func 0) :
-    bShift (SubTerm.func (L := L) (μ:= μ) (n := n) f ![]) = SubTerm.func f ![] := by simp[bShift_func]
-
-lemma bShift_func1 (f : L.func 1) {t : SubTerm L μ n} {t'} (h : bShift t = t'):
-    bShift (SubTerm.func f ![t]) = SubTerm.func f ![t'] := by simp[←h, bShift_func]; funext x; simp
-
-lemma bShift_func2 (f : L.func 2) {t₁ t₂ : SubTerm L μ n} {t₁' t₂'}
-  (h₁ : bShift t₁ = t₁') (h₂ : bShift t₂ = t₂') :
-    bShift (SubTerm.func f ![t₁, t₂]) = SubTerm.func f ![t₁', t₂'] :=
-  by simp[←h₁, ←h₂, bShift_func]; funext x; cases x using Fin.cases <;> simp
-
-lemma bShift_func3 (f : L.func 3) {t₁ t₂ t₃ : SyntacticSubTerm L n} {t₁' t₂' t₃'}
-  (h₁ : bShift t₁ = t₁') (h₂ : bShift t₂ = t₂') (h₃ : bShift t₃ = t₃') :
-    bShift (SubTerm.func f ![t₁, t₂, t₃]) = SubTerm.func f ![t₁', t₂', t₃'] := by
-  simp[←h₁, ←h₂, ←h₃, bShift_func]; funext x;
-  cases' x using Fin.cases with x <;> simp;
-  cases' x using Fin.cases with x <;> simp
-
-lemma bShift_subst {t : SyntacticSubTerm L (n + 1)} {u t' u'}
-  (ht : bShift t = t') (hu : bShift u = u') :
-    bShift (subst u t) = subst u' t' := by
-  simp[←ht, ←hu, bShift, SubTerm.subst, map, bind_bind]; congr; funext x
-  cases' x using Fin.lastCases with x <;> simp[Fin.succ_castSucc]
-
-lemma func1_congr (f : L.func 1) {t t' : SyntacticSubTerm L n} (h : t = t'):
-    SubTerm.func f ![t] = SubTerm.func f ![t'] := by simp[←h]
-
-lemma func2_congr (f : L.func 2) {t₁ t₂ t₁' t₂' : SyntacticSubTerm L n}
-  (h₁ : t₁ = t₁') (h₂ : t₂ = t₂') :
-    SubTerm.func f ![t₁, t₂] = SubTerm.func f ![t₁', t₂'] :=
-  by simp[←h₁, ←h₂]
-
-lemma func3_congr (f : L.func 3) {t₁ t₂ t₃ t₁' t₂' t₃' : SyntacticSubTerm L n}
-  (h₁ : t₁ = t₁') (h₂ : t₂ = t₂') (h₃ : t₃ = t₃') :
-    SubTerm.func f ![t₁, t₂, t₃] = SubTerm.func f ![t₁', t₂', t₃'] := by
-  simp[←h₁, ←h₂, ←h₃]
+lemma func_congr  {k} (f : L.func k) {v₁ v₂ : Fin k → SyntacticSubTerm L n} (h : v₁ = v₂):
+    func f v₁ = func f v₂ := by simp[←h]
 
 lemma free_congr_eq {t t' : SyntacticSubTerm L (n + 1)} {s} (e : t = t') (h : free t' = s) :
   free t = s := Eq.trans (congr_arg _ e) h
-
-lemma subst_congr_eq {s s' : SubTerm L μ n} {t t' u} (es : s = s') (et : t = t') (h : subst s' t' = u) :
-  subst s t = u := Eq.trans (congr_arg₂ SubTerm.subst es et) h
 
 lemma shift_congr_eq {t t' : SyntacticSubTerm L n} {u} (e : t = t') (h : shift t' = u) :
   shift t = u := Eq.trans (congr_arg _ e) h
@@ -138,10 +91,6 @@ variable (c : Const L)
 
 @[simp] lemma free_const :
     free (c : SyntacticSubTerm L (n + 1)) = c :=
-  by simp
-
-@[simp] lemma subst_const {s} :
-    subst s (c : SubTerm L μ (n + 1)) = c :=
   by simp
 
 @[simp] lemma substs_const {n'} {w : Fin n → SubTerm L μ n'} :
@@ -165,9 +114,53 @@ end
 
 end lemmata
 
+partial def resultSubsts {L : Q(Language.{u})} {k n : Q(ℕ)} (w : Q(Fin $k → SyntacticSubTerm $L $n)) :
+    (t : Q(SyntacticSubTerm $L $k)) → MetaM ((res : Q(SyntacticSubTerm $L $n)) × Q(substs $w $t = $res))
+  | ~q(#$x)                          => do
+    let ⟨t, ht⟩ ← vectorQNth (u := u) k w x
+    return ⟨t, q(substs_bvar_of_eq $ht)⟩
+  | ~q(&$x)                          => pure ⟨q(&$x), q(substs_fvar $w $x)⟩
+  | ~q(func (arity := $arity) $f $v) => do
+    let ⟨v', ve⟩ ← resultVectorOfResultFun (u := u) (v := u)
+      (α := q(SyntacticSubTerm $L $k)) (β := q(SyntacticSubTerm $L $n))
+      q(substs $w) (resultSubsts w) arity v
+    return ⟨q(func $f $v'), q(substs_func_of_eq $f $ve)⟩
+  | ~q(Operator.const $c)            => pure ⟨q(Operator.const $c), q(substs_const $c)⟩
+  | ~q(substs (n := $l) $v $t)       => do
+    let ⟨v', ve⟩ ← resultVectorOfResultFun (u := u) (v := u)
+      (α := q(SyntacticSubTerm $L $k)) (β := q(SyntacticSubTerm $L $n))
+      q(@SubTerm.substs $L ℕ $k $n $w) (resultSubsts w) l v
+    let ⟨p', pe⟩ ← resultSubsts v' t
+    return ⟨p', q(substs_substs_of_eq $ve $pe)⟩
+  | ~q($t)                           => pure ⟨q(substs $w $t), q(rfl)⟩
+
+partial def resultShift {L : Q(Language.{u})} {n : Q(ℕ)} : (t : Q(SyntacticSubTerm $L $n)) →
+    MetaM ((res : Q(SyntacticSubTerm $L $n)) × Q(SubTerm.shift $t = $res))
+  | ~q(#$x)                          => pure ⟨q(#$x), q(SubTerm.shift_bvar $x)⟩
+  | ~q(&$x)                          =>  do
+    let z ← natAppFunQ Nat.succ x
+    let e := q(SubTerm.shift_fvar (L := $L) (n := $n) $x)
+    return ⟨q(&$z), e⟩
+  | ~q(func (arity := $arity) $f $v) => do
+    let ⟨v', ve'⟩ ← resultVectorOfResultFun (u := u) (v := u)
+      (α := q(SyntacticSubTerm $L $n)) (β := q(SyntacticSubTerm $L $n))
+      q(@shift $L $n) resultShift arity v
+    let e : Q(SyntacticSubTerm $L $n) := q(func $f $v')
+    return ⟨e, q(shift_func_of_eq $f $ve')⟩
+  | ~q(substs (n := $k) $w $t)       => do
+    let ⟨t', te⟩ ← resultShift (L := L) (n := k) t
+    let ⟨w', we⟩ ← resultVectorOfResultFun (u := u) (v := u)
+      (α := q(SyntacticSubTerm $L $n)) (β := q(SyntacticSubTerm $L $n))
+      q(@SubTerm.shift $L $n) resultShift k w
+    let ⟨t'', t'e⟩ ← resultSubsts w' t'
+    return ⟨t'', q(shift_substs_of_eq $te $we $t'e)⟩
+  | ~q(SubTerm.Operator.const $c)    => pure ⟨q(SubTerm.Operator.const $c), q(shift_const $c)⟩
+  | ~q($t)                           => do
+    return ⟨q(shift $t), q(rfl)⟩
+
 partial def resultFree {L : Q(Language.{u})} {n : Q(ℕ)} : (t : Q(SyntacticSubTerm $L ($n + 1))) →
     MetaM ((res : Q(SyntacticSubTerm $L $n)) × Q(SubTerm.free $t = $res))
-  | ~q(#$x)                              => do
+  | ~q(#$x)                          => do
     let n ←whnf n 
     let some nval := n.natLit? | throwError f!"Fail: natLit: {n}"
     let some xval := (← finQVal (n := q(.succ $n)) x) | throwError f!"Fail: FinQVal {x}"
@@ -179,114 +172,49 @@ partial def resultFree {L : Q(Language.{u})} {n : Q(ℕ)} : (t : Q(SyntacticSubT
       let e := q(free_bvar_of_lt (L := $L) $x $lt)
       let z : Q(Fin $n) ← Lean.Expr.ofNat q(Fin $n) xval
       return ⟨q(#$z), e⟩
-  | ~q(&$x)                              => do
+  | ~q(&$x)                          => do
     let z ← natAppFunQ Nat.succ x
     let e : Expr := q(SubTerm.free_fvar (L := $L) (n := $n) $x)
     return ⟨q(&$z), e⟩
-  | ~q(SubTerm.func $f ![])              => pure ⟨q(SubTerm.func $f ![]), q(free_func0 $f)⟩
-  | ~q(SubTerm.func $f ![$t])            => do
-    let ⟨tn, e⟩ ← resultFree (L := L) (n := n) t
-    return ⟨q(SubTerm.func $f ![$tn]), q(free_func1 $f $e)⟩
-  | ~q(SubTerm.func $f ![$t₁, $t₂])      => do
-    let ⟨tn₁, e₁⟩ ← resultFree (L := L) (n := n) t₁
-    let ⟨tn₂, e₂⟩ ← resultFree (L := L) (n := n) t₂
-    return ⟨q(SubTerm.func $f ![$tn₁, $tn₂]), q(free_func2 $f $e₁ $e₂)⟩
-  | ~q(SubTerm.func $f ![$t₁, $t₂, $t₃]) => do
-    let ⟨tn₁, e₁⟩ ← resultFree (L := L) (n := n) t₁
-    let ⟨tn₂, e₂⟩ ← resultFree (L := L) (n := n) t₂
-    let ⟨tn₃, e₃⟩ ← resultFree (L := L) (n := n) t₃
-    return ⟨q(SubTerm.func $f ![$tn₁, $tn₂, $tn₃]), q(free_func3 $f $e₁ $e₂ $e₃)⟩
-  | ~q(SubTerm.Operator.const $c) => pure ⟨q(SubTerm.Operator.const $c), q(free_const _)⟩
-  | ~q($t)                               => do
+  | ~q(func (arity := $arity) $f $v) => do
+    let ⟨v', ve'⟩ ← resultVectorOfResultFun (u := u) (v := u)
+      (α := q(SyntacticSubTerm $L ($n + 1))) (β := q(SyntacticSubTerm $L $n))
+      q(@free $L $n) resultFree arity v
+    let e : Q(SyntacticSubTerm $L $n) := q(func $f $v')
+    return ⟨e, q(free_func_of_eq $f $ve')⟩
+  | ~q(substs (n := $k) $w $t)       => do
+    let ⟨t', te⟩ ← resultShift (L := L) (n := k) t
+    let ⟨w', we⟩ ← resultVectorOfResultFun (u := u) (v := u)
+      (α := q(SyntacticSubTerm $L ($n + 1))) (β := q(SyntacticSubTerm $L $n))
+      q(@SubTerm.free $L $n) resultFree k w
+    let ⟨t'', t'e⟩ ← resultSubsts w' t'
+    return ⟨t'', q(free_substs_of_eq $te $we $t'e)⟩
+  | ~q(SubTerm.Operator.const $c)    => pure ⟨q(SubTerm.Operator.const $c), q(free_const _)⟩
+  | ~q($t)                           => do
     return ⟨q(SubTerm.free $t), q(rfl)⟩
-
--- TODO: replace with `substs`
-partial def resultSubst {L : Q(Language.{u})} {n : Q(ℕ)} (s : Q(SyntacticSubTerm $L $n)) :
-    (t : Q(SyntacticSubTerm $L ($n + 1))) →
-    MetaM ((res : Q(SyntacticSubTerm $L $n)) × Q(SubTerm.subst $s $t = $res))
-  | ~q(#$x)                              => do
-    let n ←whnf n 
-    let some nval := n.natLit? | throwError f!"Fail: natLit: {n}"
-    let some xval := (← finQVal (n := q(.succ $n)) x) | throwError f!"Fail: FinQVal {x}"
-    if xval = nval then
-      return ⟨q($s), (q(subst_bvar_last $n $s) : Expr)⟩
-    else
-      let lt ← decideTQ q(($x).val < $n)
-      let e := q(free_bvar_of_lt (L := $L) $x $lt)
-      let z : Q(Fin $n) ← Lean.Expr.ofNat q(Fin $n) xval
-      return ⟨q(#$z), e⟩
-  | ~q(&$x)                              => pure ⟨q(&$x), q(SubTerm.subst_fvar _ _)⟩
-  | ~q(SubTerm.func $f ![])              => pure ⟨q(SubTerm.func $f ![]), q(subst_func0 $f)⟩
-  | ~q(SubTerm.func $f ![$t])            => do
-    let ⟨tn, e⟩ ← resultSubst (L := L) (n := n) s t
-    return ⟨q(SubTerm.func $f ![$tn]), q(subst_func1 $f $e)⟩
-  | ~q(SubTerm.func $f ![$t₁, $t₂])      => do
-    let ⟨tn₁, e₁⟩ ← resultSubst (L := L) (n := n) s t₁
-    let ⟨tn₂, e₂⟩ ← resultSubst (L := L) (n := n) s t₂
-    return ⟨q(SubTerm.func $f ![$tn₁, $tn₂]), q(subst_func2 $f $e₁ $e₂)⟩
-  | ~q(SubTerm.func $f ![$t₁, $t₂, $t₃]) => do
-    let ⟨tn₁, e₁⟩ ← resultSubst (L := L) (n := n) s t₁
-    let ⟨tn₂, e₂⟩ ← resultSubst (L := L) (n := n) s t₂
-    let ⟨tn₃, e₃⟩ ← resultSubst (L := L) (n := n) s t₃
-    return ⟨q(SubTerm.func $f ![$tn₁, $tn₂, $tn₃]), q(subst_func3 $f $e₁ $e₂ $e₃)⟩
-  | ~q(SubTerm.Operator.const $c) => pure ⟨q(SubTerm.Operator.const $c), q(subst_const $c)⟩
-  | ~q($t)                               => do
-    return ⟨q(SubTerm.subst $s $t), q(rfl)⟩
-
-partial def resultShift {L : Q(Language.{u})} {n : Q(ℕ)} : (t : Q(SyntacticSubTerm $L $n)) →
-    MetaM ((res : Q(SyntacticSubTerm $L $n)) × Q(SubTerm.shift $t = $res))
-  | ~q(#$x)                              => pure ⟨q(#$x), q(SubTerm.shift_bvar $x)⟩
-  | ~q(&$x)                              =>  do
-    let z ← natAppFunQ Nat.succ x
-    let e := q(SubTerm.shift_fvar (L := $L) (n := $n) $x)
-    return ⟨q(&$z), e⟩
-  | ~q(SubTerm.func $f ![])              => pure ⟨q(SubTerm.func $f ![]), q(shift_func0 $f)⟩
-  | ~q(SubTerm.func $f ![$t])            => do
-    let ⟨tn, e⟩ ← resultShift (L := L) (n := n) t
-    return ⟨q(SubTerm.func $f ![$tn]), q(shift_func1 $f $e)⟩
-  | ~q(SubTerm.func $f ![$t₁, $t₂])      => do
-    let ⟨tn₁, e₁⟩ ← resultShift (L := L) (n := n) t₁
-    let ⟨tn₂, e₂⟩ ← resultShift (L := L) (n := n) t₂
-    return ⟨q(SubTerm.func $f ![$tn₁, $tn₂]), q(shift_func2 $f $e₁ $e₂)⟩
-  | ~q(SubTerm.func $f ![$t₁, $t₂, $t₃]) => do
-    let ⟨tn₁, e₁⟩ ← resultShift (L := L) (n := n) t₁
-    let ⟨tn₂, e₂⟩ ← resultShift (L := L) (n := n) t₂
-    let ⟨tn₃, e₃⟩ ← resultShift (L := L) (n := n) t₃
-    return ⟨q(SubTerm.func $f ![$tn₁, $tn₂, $tn₃]), q(shift_func3 $f $e₁ $e₂ $e₃)⟩
-  | ~q(SubTerm.subst $t₁ $t₂)            => do
-    let ⟨tn₁, e₁⟩ ← resultShift (L := L) (n := n) t₁
-    let ⟨tn₂, e₂⟩ ← resultShift (L := L) (n := q(.succ $n)) t₂
-    return ⟨q(SubTerm.subst $tn₁ $tn₂), q(shift_subst $e₂ $e₁)⟩
-  | ~q(SubTerm.Operator.const $c) => pure ⟨q(SubTerm.Operator.const $c), q(shift_const $c)⟩
-  | ~q($t)                               => do
-    return ⟨q(shift $t), q(rfl)⟩
 
 partial def resultBShift {L : Q(Language.{u})} {n : Q(ℕ)} : (t : Q(SyntacticSubTerm $L $n)) →
     MetaM ((res : Q(SyntacticSubTerm $L ($n + 1))) × Q(bShift $t = $res))
-  | ~q(#$x)                              => do
-    let z ← natAppFunQ Nat.succ x
+  | ~q(#$x)                          => do
+    let some xval := (← finQVal (n := q(.succ $n)) x) | throwError f!"Fail: FinQVal {x}"
+    let z : Q(Fin ($n + 1)) ← Lean.Expr.ofNat q(Fin ($n + 1)) (xval + 1)
     let e := q(SubTerm.bShift_bvar (L := $L) (μ := ℕ) (n := $n) $x)
-    return ⟨q(&$z), e⟩
-  | ~q(&$x)                              => pure ⟨q(&$x), q(SubTerm.bShift_fvar $x)⟩
-  | ~q(SubTerm.func $f ![])              => pure ⟨q(SubTerm.func $f ![]), q(bShift_func0 $f)⟩
-  | ~q(SubTerm.func $f ![$t])            => do
-    let ⟨tn, e⟩ ← resultBShift (L := L) (n := n) t
-    return ⟨q(SubTerm.func $f ![$tn]), q(bShift_func1 $f $e)⟩
-  | ~q(SubTerm.func $f ![$t₁, $t₂])      => do
-    let ⟨tn₁, e₁⟩ ← resultBShift (L := L) (n := n) t₁
-    let ⟨tn₂, e₂⟩ ← resultBShift (L := L) (n := n) t₂
-    return ⟨q(SubTerm.func $f ![$tn₁, $tn₂]), q(bShift_func2 $f $e₁ $e₂)⟩
-  | ~q(SubTerm.func $f ![$t₁, $t₂, $t₃]) => do
-    let ⟨tn₁, e₁⟩ ← resultBShift (L := L) (n := n) t₁
-    let ⟨tn₂, e₂⟩ ← resultBShift (L := L) (n := n) t₂
-    let ⟨tn₃, e₃⟩ ← resultBShift (L := L) (n := n) t₃
-    return ⟨q(SubTerm.func $f ![$tn₁, $tn₂, $tn₃]), q(bShift_func3 $f $e₁ $e₂ $e₃)⟩
-  | ~q(SubTerm.subst $t₁ $t₂)            => do
-    let ⟨tn₁, e₁⟩ ← resultBShift (L := L) (n := n) t₁
-    let ⟨tn₂, e₂⟩ ← resultBShift (L := L) (n := q(.succ $n)) t₂
-    return ⟨q(SubTerm.subst $tn₁ $tn₂), q(bShift_subst $e₂ $e₁)⟩
-  | ~q(SubTerm.Operator.const $c) => pure ⟨q(SubTerm.Operator.const $c), q(bShift_const $c)⟩
-  | ~q($t)                               => do
+    return ⟨q(#$z), e⟩
+  | ~q(&$x)                          => pure ⟨q(&$x), q(SubTerm.bShift_fvar $x)⟩
+  | ~q(func (arity := $arity) $f $v) => do
+    let ⟨v', ve'⟩ ← resultVectorOfResultFun (u := u) (v := u)
+      (α := q(SyntacticSubTerm $L $n)) (β := q(SyntacticSubTerm $L ($n + 1)))
+      q(@bShift $L ℕ $n) resultBShift arity v
+    let e : Q(SyntacticSubTerm $L ($n + 1)) := q(func $f $v')
+    return ⟨e, q(bShift_func_of_eq $f $ve')⟩
+  | ~q(substs (n := $k) $w $t)       => do
+    let ⟨w', we⟩ ← resultVectorOfResultFun (u := u) (v := u)
+      (α := q(SyntacticSubTerm $L $n)) (β := q(SyntacticSubTerm $L ($n + 1)))
+      q(@SubTerm.bShift $L ℕ $n) resultBShift k w
+    let ⟨t', te⟩ ← resultSubsts w' t
+    return ⟨t', q(bShift_substs_of_eq $we $te)⟩
+  | ~q(SubTerm.Operator.const $c)    => pure ⟨q(SubTerm.Operator.const $c), q(bShift_const $c)⟩
+  | ~q($t)                           => do
     return ⟨q(bShift $t), q(rfl)⟩
 
 inductive NumeralUnfoldOption
@@ -305,7 +233,7 @@ partial def natLitResult {L : Q(Language.{u})}
       match z with
       | ~q(0)      => return ⟨q(natLit $L 0), q(rfl)⟩
       | ~q(1)      => return ⟨q(natLit $L 1), q(rfl)⟩
-      | ~q(.succ $ .succ $z) => do
+      | ~q(.succ $ .succ $z)       => do
         let z' ← natAppFunQ Nat.succ z
         let e := q(@rfl _ (@Operator.const $L ℕ $n (natLit $L (.succ (.succ $z)))))
         return ⟨q(func Language.Add.add ![natLit $L $z', natLit $L 1]), e⟩
@@ -322,58 +250,48 @@ partial def natLitResult {L : Q(Language.{u})}
 
 partial def result (tp : NumeralUnfoldOption) {L : Q(Language.{u})} {n : Q(ℕ)} : (t : Q(SyntacticSubTerm $L $n)) →
     MetaM ((res : Q(SyntacticSubTerm $L $n)) × Q($t = $res))
-  | ~q(#$x)                                           => pure ⟨q(#$x), q(rfl)⟩
-  | ~q(&$x)                                           => pure ⟨q(&$x), q(rfl)⟩
-  | ~q(SubTerm.func $f ![])                           => pure ⟨q(SubTerm.func $f ![]), q(rfl)⟩
-  | ~q(SubTerm.func $f ![$t])                         => do
-    let ⟨tn, e⟩ ← result tp (L := L) (n := n) t
-    return ⟨q(SubTerm.func $f ![$tn]), q(func1_congr $f $e)⟩
-  | ~q(SubTerm.func $f ![$t₁, $t₂])                   => do
-    let ⟨tn₁, e₁⟩ ← result tp (L := L) (n := n) t₁
-    let ⟨tn₂, e₂⟩ ← result tp (L := L) (n := n) t₂
-    return ⟨q(SubTerm.func $f ![$tn₁, $tn₂]), q(func2_congr $f $e₁ $e₂)⟩
-  | ~q(SubTerm.func $f ![$t₁, $t₂, $t₃])              => do
-    let ⟨tn₁, e₁⟩ ← result tp (L := L) (n := n) t₁
-    let ⟨tn₂, e₂⟩ ← result tp (L := L) (n := n) t₂
-    let ⟨tn₃, e₃⟩ ← result tp (L := L) (n := n) t₃
-    return ⟨q(SubTerm.func $f ![$tn₁, $tn₂, $tn₃]), q(func3_congr $f $e₁ $e₂ $e₃)⟩
-  | ~q(free $t)                                       => do
+  | ~q(#$x)                          => pure ⟨q(#$x), q(rfl)⟩
+  | ~q(&$x)                          => pure ⟨q(&$x), q(rfl)⟩
+  | ~q(func (arity := $arity) $f $v) => do
+    let ⟨vn, ve⟩ ← resultVectorOfResult (α := q(SyntacticSubTerm $L $n)) (u := u) (result tp) arity v
+    let e : Q(SyntacticSubTerm $L $n) := q(func $f $vn)
+    return ⟨e, q(func_congr $f $ve)⟩
+  | ~q(free $t)                      => do
     let ⟨tn, e⟩ ← result tp (L := L) (n := q(.succ $n)) t
     let ⟨tnn, ee⟩ ← resultFree (L := L) (n := n) tn
     return ⟨q($tnn), q(free_congr_eq $e $ee)⟩
-  | ~q(subst $s $t)                                   => do
-    let ⟨tn, te⟩ ← result tp (L := L) (n := q(.succ $n)) t
-    let ⟨sn, se⟩ ← result tp (L := L) (n := q($n)) s
-    let ⟨tnn, ee⟩ ← resultSubst (L := L) (n := n) sn tn
-    return ⟨q($tnn), q(subst_congr_eq $se $te $ee)⟩
-  | ~q(shift $t)                                      => do
-    let ⟨tn, e⟩ ← result tp (L := L) (n := q($n)) t
-    let ⟨tnn, ee⟩ ← resultShift (L := L) (n := n) tn
-    return ⟨q($tnn), q(shift_congr_eq $e $ee)⟩
+  | ~q(substs (n := $k) $w $t)       => do
+    let ⟨t', te⟩ ← result tp (L := L) (n := k) t
+    let ⟨w', we⟩ ← resultVectorOfResult (α := q(SyntacticSubTerm $L $n)) (u := u) (result tp) k w
+    let ⟨e, t''⟩ ← resultSubsts (u := u) w' t'
+    return ⟨e, q(substs_eq_of_eq $we $te $t'')⟩
+  | ~q(shift $t)                     => do
+    let ⟨t', te⟩ ← result tp (L := L) (n := q($n)) t
+    let ⟨t'', tee⟩ ← resultShift (L := L) (n := n) t'
+    return ⟨q($t''), q(shift_congr_eq $te $tee)⟩
   | ~q(SubTerm.Operator.const $ natLit (hz := $hz) (ho := $ho) (ha := $ha) $z) => natLitResult hz ho ha n tp z
-  | ~q($t)                                            => pure ⟨q($t), q(rfl)⟩
-
-private inductive ResultTest (α : Type u) : (a : α) → Type u
-  | result : (a b : α) → a = b → ResultTest α a
+  | ~q($t)                           => pure ⟨q($t), q(rfl)⟩
 
 elab "dbg" : tactic => do
   let goalType ← Elab.Tactic.getMainTarget
   let some ⟨.succ u, ty⟩ ← checkSortQ' goalType | throwError "error: not a type"
-  let ~q(ResultTest (SyntacticSubTerm $L $n) $t) := ty | throwError "error: not a type"
+  let ~q(DbgResult (SyntacticSubTerm $L $n) $t) := ty | throwError "error: not a type"
   logInfo m!"t = {t}"
   let t : Q(SyntacticSubTerm $L $n) ← withReducible <| whnf t
-  let ⟨tn, e⟩ ← result NumeralUnfoldOption.unfoldSucc (L := L) (n := n) t
+  let ⟨tn, e⟩ ← result NumeralUnfoldOption.none (L := L) (n := n) t
+  let ⟨tnbs, ebs⟩ ← resultBShift (L := L) (n := n) tn
   logInfo m!"tn = {tn}"
-  logInfo m!"e = {e}"
-  let c : Q(ResultTest (SyntacticSubTerm $L $n) $t) := (q(ResultTest.result ($t) $tn $e) : Expr)
+  logInfo m!"tnbs = {tnbs}"
+  --logInfo m!"e = {e}"
+  let c : Q(DbgResult (SyntacticSubTerm $L $n) $t) := (q(DbgResult.intro ($t) $tn $e) : Expr)
   Lean.Elab.Tactic.closeMainGoal c
 
-example {t : SyntacticSubTerm Language.oring 13} : ResultTest (SyntacticSubTerm Language.oring 12)
-    (shift $ subst &99 T“(!t) + (2 * !(shift T“#2 + 9”)) + &7”) :=
+example {t : SyntacticSubTerm Language.oring 2} : DbgResult (SyntacticSubTerm Language.oring 12)
+    (shift $ substs ![substs ![T“6”, T“&7”] t, T“3 + &6”] T“(!t) + (#0 * !(shift T“#1 + 9 * #1”)) + &7”) :=
   by dbg
 
-example {t : SyntacticSubTerm Language.oring 13} (z : ℕ) : ResultTest (SyntacticSubTerm Language.oring 12)
-    T“8” :=
+example (t : SyntacticSubTerm Language.oring 3) : DbgResult (SyntacticSubTerm Language.oring 12)
+    T“((#0 + #1 + #2 + 8 * !t) ⟦#2, 7, 4⟧ ⟦4, 4, 5⟧) * 8” :=
   by dbg
 
 example : 1 ≠ 2 := of_decide_eq_true rfl
